theories/Transform/ReadOffPreproof.v
@@ -12,47 +12,45 @@ Set Default Proof Using "Type".
 Module RO := ReadOff.
 
 Section Packaging.
-  (** For now we package the raw read-off graph as a preproof with a trivial
-      local rule. The next step will replace `Rule` by the vertex-typing rule
-      relation (`jTyV/jEqV/jSubV`). *)
+  (** Package the raw read-off graph as a rooted preproof.
+
+      For now, the local rule is trivial (`True`). This step exists to move from
+      “maps representing a cyclic graph” to the project’s standard `preproof`
+      structure.
+
+      Next step: replace `Rule` by the vertex-typing/equality/substitution rule
+      relation (`jTyV/jEqV/jSubV`) and prove `pp_rule_ok` by construction.
+  *)
 
   Definition Judgement : Type := RO.node.
   Definition Rule (_ : Judgement) (_ : list Judgement) : Prop := True.
 
-  Definition verts_of (n : nat) : gset nat :=
-    list_to_set (seq 0 n).
+  Definition verts_of (b : RO.builder) : gset nat :=
+    dom (RO.b_label b).
 
   Definition succ_of (b : RO.builder) (v : nat) : list nat :=
-    filter (fun w => bool_decide (w < RO.b_next b))
+    filter (fun w => bool_decide (w ∈ verts_of b))
       (default [] (RO.b_succ b !! v)).
 
   Definition label_of (b : RO.builder) (v : nat) : RO.node :=
     default (RO.nVar 0) (RO.b_label b !! v).
 
   Lemma succ_of_closed (b : RO.builder) (v : nat) :
-    Forall (fun w => w ∈ verts_of (RO.b_next b)) (succ_of b v).
+    Forall (fun w => w ∈ verts_of b) (succ_of b v).
   Proof.
     apply Forall_forall.
     intros w Hw.
     unfold succ_of in Hw.
     apply elem_of_list_filter in Hw.
-    destruct Hw as [Hw Hlt].
-    apply bool_decide_true in Hlt.
-    unfold verts_of.
-    apply elem_of_list_to_set.
-    (* `w < b_next b` implies `w ∈ seq 0 (b_next b)` *)
-    apply (proj2 (elem_of_seq 0 (RO.b_next b) w)).
-    lia.
+    destruct Hw as [_ Hw].
+    now apply bool_decide_true in Hw.
   Qed.
 
   Program Definition graph_of (b : RO.builder) : FiniteDigraph.fin_digraph nat :=
-    {| FiniteDigraph.verts := verts_of (RO.b_next b);
-       FiniteDigraph.succ := succ_of b;
-    |}.
+    {| FiniteDigraph.verts := verts_of b;
+       FiniteDigraph.succ := succ_of b |}.
   Next Obligation.
     intros b v Hv.
-    unfold FiniteDigraph.succ.
-    simpl.
     exact (succ_of_closed b v).
   Qed.
 
@@ -61,72 +59,70 @@ Section Packaging.
        Preproof.pp_label := label_of b;
        Preproof.pp_rule_ok := fun _ _ => I |}.
 
-  (* Basic monotonicity: compilation never decreases `b_next`. *)
-  Lemma put_preserves_next (v : nat) (lbl : RO.node) (succs : list nat) (b : RO.builder) :
-    RO.b_next (RO.put v lbl succs b) = RO.b_next b.
-  Proof. reflexivity. Qed.
-
-  Lemma put_fix_ty_preserves_next (v vA : nat) (b : RO.builder) :
-    RO.b_next (RO.put_fix_ty v vA b) = RO.b_next b.
-  Proof. reflexivity. Qed.
-
-  Lemma fresh_increases_next (b : RO.builder) (v : nat) (b' : RO.builder) :
-    RO.fresh b = (v, b') -> RO.b_next b' = S (RO.b_next b).
+  Lemma compile_tm_root_label (fuel : nat) (ρ : RO.back_env) (t : Term.Syntax.tm)
+      (b : RO.builder) (root : nat) (b' : RO.builder) :
+    RO.compile_tm fuel ρ t b = (root, b') ->
+    is_Some (RO.b_label b' !! root).
   Proof.
-    unfold RO.fresh.
-    intro H.
-    inversion H.
-    reflexivity.
-  Qed.
-
-  Lemma compile_tm_next_ge (fuel : nat) (ρ : RO.back_env) (t : Term.Syntax.tm)
-      (b : RO.builder) (v : nat) (b' : RO.builder) :
-    RO.compile_tm fuel ρ t b = (v, b') ->
-    RO.b_next b <= RO.b_next b'.
-  Proof.
-    revert ρ t b v b'.
-    induction fuel as [|fuel IH]; intros ρ t b v b' H;
+    revert ρ t b root b'.
+    induction fuel as [|fuel IH]; intros ρ t b root b' H;
       simpl in H.
     - (* fuel = 0 *)
       destruct (RO.fresh b) as [v0 b0] eqn:Hfresh.
       inversion H; subst.
-      rewrite (fresh_increases_next _ _ _ Hfresh).
-      lia.
+      unfold RO.put.
+      simpl.
+      rewrite lookup_insert.
+      eexists.
+      reflexivity.
     - (* fuel = S fuel *)
-      destruct t; simpl in H.
-      all: repeat
-        match goal with
-        | Hf : RO.fresh _ = _ |- _ =>
-            apply fresh_increases_next in Hf
-        end.
-      all: try (repeat (destruct (RO.fresh b) as [v0 b0] eqn:Hfresh; clear Hfresh));
-        (* For the remaining cases we can simply use that the result builder is
-           obtained from the initial one by a sequence of `fresh` allocations. *)
-        admit.
-  Admitted.
+      destruct t; try (destruct (RO.fresh b) as [v0 b0] eqn:Hfresh; inversion H; subst;
+        unfold RO.put; simpl; rewrite lookup_insert; eexists; reflexivity).
+      all: try (destruct (RO.fresh b) as [v0 b0] eqn:Hfresh;
+        (* the remaining cases perform recursive compilation but always end by `put v0 ...` *)
+        repeat (destruct (RO.compile_tm fuel _ _ _ ) as [vx bx] eqn:?);
+        inversion H; subst; unfold RO.put; simpl; rewrite lookup_insert; eexists; reflexivity).
+      (* tApp case *)
+      + (* tApp *)
+        destruct (RO.app_view (Term.Syntax.tApp t1 t2)) as [h args] eqn:Hview.
+        destruct h.
+        * (* head is a variable *)
+          destruct (nth_error ρ x) as [[target|]|] eqn:Hnth.
+          -- (* backlink case *)
+             (* after allocating the backlink vertex we always `put` it *)
+             repeat (destruct (RO.compile_tm fuel ρ _ _) as [vx bx] eqn:?);
+             repeat (destruct (RO.fresh _) as [vx bx] eqn:?);
+             inversion H; subst; unfold RO.put; simpl; rewrite lookup_insert; eexists; reflexivity.
+          -- (* non-backlink *)
+             destruct (RO.fresh b) as [v0 b0] eqn:Hfresh.
+             repeat (destruct (RO.compile_tm fuel _ _ _ ) as [vx bx] eqn:?);
+             inversion H; subst; unfold RO.put; simpl; rewrite lookup_insert; eexists; reflexivity.
+          -- (* non-backlink *)
+             destruct (RO.fresh b) as [v0 b0] eqn:Hfresh.
+             repeat (destruct (RO.compile_tm fuel _ _ _ ) as [vx bx] eqn:?);
+             inversion H; subst; unfold RO.put; simpl; rewrite lookup_insert; eexists; reflexivity.
+        * (* head is not a variable *)
+          destruct (RO.fresh b) as [v0 b0] eqn:Hfresh.
+          repeat (destruct (RO.compile_tm fuel _ _ _ ) as [vx bx] eqn:?);
+          inversion H; subst; unfold RO.put; simpl; rewrite lookup_insert; eexists; reflexivity.
+  Qed.
 
-  Lemma compile_tm_root_in (t : Term.Syntax.tm) (root : nat) (b : RO.builder) :
+  Lemma read_off_root_in (t : Term.Syntax.tm) (root : nat) (b : RO.builder) :
     RO.read_off_raw t = (root, b) ->
     root ∈ verts (graph_of b).
   Proof.
     intro H.
     unfold RO.read_off_raw in H.
-    unfold verts.
-    simpl.
-    unfold RO.compile_tm in H.
-    (* We only need the easy fact: `root < b_next b`. *)
-    pose proof (compile_tm_next_ge (fuel := Term.Syntax.size t) (ρ := []) (t := t)
-                 (b := RO.empty_builder) (v := root) (b' := b)) as Hge.
-    specialize (Hge H).
-    unfold verts_of.
-    apply elem_of_list_to_set.
-    apply (proj2 (elem_of_seq 0 (RO.b_next b) root)).
-    lia.
+    apply elem_of_dom.
+    apply (compile_tm_root_label (fuel := Term.Syntax.size t) (ρ := [])
+             (t := t) (b := RO.empty_builder) (root := root) (b' := b)).
+    exact H.
   Qed.
 
-  Definition rooted_preproof_of (t : Term.Syntax.tm) : @Preproof.rooted_preproof Judgement Rule nat _ _ :=
+  Definition rooted_preproof_of (t : Term.Syntax.tm)
+      : @Preproof.rooted_preproof Judgement Rule nat _ _ :=
     let '(root, b) := RO.read_off_raw t in
     {| Preproof.rpp_proof := preproof_of b;
        Preproof.rpp_root := root;
-       Preproof.rpp_root_in := (compile_tm_root_in t root b eq_refl) |}.
+       Preproof.rpp_root_in := (read_off_root_in t root b eq_refl) |}.
 End Packaging.
